Tests/AxiomAudit.lean
@@ -140,6 +140,7 @@ elab "#assert_axioms " id:ident : command => do
 
 #assert_axioms BtcVerified.Tx.body_inputs_ne_nil
 #assert_axioms BtcVerified.Tx.isWellFormed_iff
+#assert_axioms BtcVerified.Tx.WellFormed.outputs_length_le
 #assert_axioms BtcVerified.Coin.isMature_iff
 #assert_axioms BtcVerified.TxBody.isFinal_iff
 #assert_axioms BtcVerified.Tx.spentCoins_length
